Generalized eq_lrt

LogicalRefinement/Stlc/InterpIrrel.lean
@@ -14,27 +14,34 @@ def Context.is_rel (Γ: Context) (n: Nat): Prop
   := ∃A, HasVar Γ n (HypKind.val type) A
 
 @[simp] def Stlc.Context.interp.eq_mod_lrt 
-  {Γ: Stlc.Context} (G G': Γ.interp) (Γ: _root_.Context): Prop
-  := ∀n: Nat, Γ.is_rel n -> eq_at G G' n
+  {Γ' Δ': Stlc.Context} (G: Γ'.interp) (D: Δ'.interp) 
+  (Γ Δ: _root_.Context): Prop
+  := ∀n: Nat, Γ.is_rel n ∧ Δ.is_rel n -> eq_at G D n
 
 theorem Stlc.Context.interp.eq_mod_lrt.extend
-    {Δ: Stlc.Context} 
+    {Γ' Δ': Stlc.Context} 
     {H: Hyp} {x: Option H.ty.stlc_ty.interp} 
-    {G G': Δ.interp} {Γ: _root_.Context}:
-  G.eq_mod_lrt G' Γ -> @eq_mod_lrt (_::Δ) (x, G) (x, G') (H::Γ)
+    {G: Γ'.interp} {D: Δ'.interp} {Γ Δ: _root_.Context}:
+  G.eq_mod_lrt D Γ Δ -> 
+  @eq_mod_lrt (_::Γ') (_::Δ') (x, G) (x, D) (H::Γ) (H::Δ)
   := by {
     intro HGG' n Hn;
     cases n with
-    | zero => rfl
+    | zero => exact ⟨rfl, rfl⟩
     | succ n => 
       apply HGG' n;
-      have ⟨A, HAn⟩ := Hn;
+      have ⟨⟨A, HAn⟩, ⟨A', HAn'⟩⟩ := Hn;
       cases HAn;
+      cases HAn';
+      constructor
+      constructor
+      assumption
       constructor
       assumption
   }
 
-theorem HasType.interp_irrel_dep {Γ a A} (H: Γ ⊢ a: expr type A) (n: Nat):
+theorem HasType.interp_irrel_dep {Γ a A} 
+  (H: Γ ⊢ a: expr type A) (n: Nat):
   a.stlc.has_dep n -> Γ.is_rel n := by {
     generalize HA': expr type A = A';
     rw [HA'] at H;
@@ -47,14 +54,19 @@ theorem HasType.interp_irrel_dep {Γ a A} (H: Γ ⊢ a: expr type A) (n: Nat):
     | _ => cases HA' <;> sorry
   }
 
-theorem HasType.interp_irrel_eq {Γ a A} {G G': Γ.stlc.interp} 
-  (H: Γ ⊢ a: expr type A) 
-  (HGG': G.eq_mod_lrt G' Γ)
-  : G.eq_mod G' a.stlc 
-  := λ_ Hn => HGG' _ (H.interp_irrel_dep _ Hn)
+theorem HasType.interp_irrel_eq {Γ Δ a A} 
+  {G: Γ.stlc.interp} {D: Δ.stlc.interp} 
+  (HΓ: Γ ⊢ a: expr type A)
+  (HΔ: Δ ⊢ a: expr type A)
+  (HGD: G.eq_mod_lrt D Γ Δ)
+  : G.eq_mod D a.stlc 
+  := λ_ Hn => 
+    HGD _ ⟨(HΓ.interp_irrel_dep _ Hn), (HΔ.interp_irrel_dep _ Hn)⟩
 
-theorem HasType.interp_irrel {Γ a A} {G G': Γ.stlc.interp} 
-  (H: Γ ⊢ a: expr type A)
-  (HGG': G.eq_mod_lrt G' Γ)
-  : H.stlc.interp G = H.stlc.interp G'
-  := H.stlc.eq_mod (H.interp_irrel_eq HGG')
+theorem HasType.interp_irrel {Γ Δ a A} 
+  {G: Γ.stlc.interp} {D: Δ.stlc.interp} 
+  (HΓ: Γ ⊢ a: expr type A)
+  (HΔ: Δ ⊢ a: expr type A)
+  (HGD: G.eq_mod_lrt D Γ Δ)
+  : HΓ.stlc.interp G = HΔ.stlc.interp D
+  := HΓ.stlc.eq_mod HΔ.stlc (HΓ.interp_irrel_eq HΔ HGD)
